src/Completeness.v
@@ -9,6 +9,7 @@ Require Import Relation_Operators.
 Require Import Coq.Setoids.Setoid.
 Require Import Typing.
 Require Import Infer.
+Require Import NewTypeVariable.
 
 Require Import LibTactics.
 
@@ -16,7 +17,8 @@ Lemma id_increases_in_w : forall (e : term) (i i' : id) (G : ctx) (t : ty) (s : 
                             getState (runInfer_id e G i) = Some i' -> i <= i'.
   Admitted.
 
-Lemma new_tv_W: ∀ (e : expr) (G : ctx) (i i’: stamp) (t : ty) (s : substitution) rs,
+Lemma new_tv_W: forall (e : term) (G : ctx) (i i': id) (t : ty) (s : substitution)
+                  rs,
     (new_tv_ctx G i) -> (runInfer_id e G i) = rs -> getState rs = Some i' ->
-    getResult rs = Some (t, s) ->
-    (new_tv_type t i’) ∧ (new_tv_subst s i’).
+    getResult rs = Some (t, s).
+
